coq/semantics: Partition log by register

Environments.v
@@ -68,11 +68,12 @@ Section Contexts.
     - exists (v, ctx); reflexivity.
   Defined.
 
-  Fixpoint ccreate (sig: list K) (f: forall k, V k) : context sig :=
-    match sig with
-    | nil => CtxEmpty
-    | cons h t => CtxCons h (f h) (ccreate t f)
-    end.
+  Fixpoint ccreate (sig: list K) (f: forall k, member k sig -> V k) : context sig :=
+    match sig return (forall k, member k sig -> V k) -> context sig with
+    | nil => fun _ => CtxEmpty
+    | cons h t => fun f => CtxCons h (f h (MemberHd h t))
+                               (ccreate t (fun k m => f k (MemberTl k h t m)))
+    end f.
 
   Fixpoint cassoc {sig} {k} (m: member k sig)
            (ctx: context sig) {struct m} : V k.
@@ -80,6 +81,35 @@ Section Contexts.
     destruct m; inversion ctx; subst; eauto.
   Defined.
 
+  Lemma cassoc_ccreate {sig} (f: forall k, _ -> V k) {k} (m: member k sig) :
+    cassoc m (ccreate sig f) = f k m.
+  Proof.
+    induction sig; cbn.
+    - pose proof (mdestruct m) as Hd; elim Hd.
+    - pose proof (mdestruct m) as [(eqn & Heq) | (m' & Heq)].
+      + destruct eqn; cbn in *; rewrite Heq.
+        reflexivity.
+      + rewrite Heq; cbn.
+        apply IHsig.
+  Qed.
+
+  Lemma ccreate_funext {sig} (f1 f2: forall k, _ -> V k):
+    (forall k m, f1 k m = f2 k m) ->
+    ccreate sig f1 = ccreate sig f2.
+  Proof.
+    induction sig; cbn.
+    - intros; reflexivity.
+    - intros Heq; rewrite Heq; eauto using f_equal.
+  Qed.
+
+  Lemma ccreate_cassoc {sig} (ctx: context sig):
+    ccreate sig (fun k m => cassoc m ctx) = ctx.
+  Proof.
+    induction sig; cbn; intros.
+    - apply context_
+    
+
+  
   Fixpoint creplace {sig} {k} (m: member k sig) (v: V k)
            (ctx: context sig) {struct m} : context sig.
     destruct m.
@@ -124,11 +154,30 @@ Record Env {K: Type}  :=
   { env_t: forall (V: esig K), Type;
     getenv: forall {V: esig K}, env_t V -> forall k, V k;
     putenv: forall {V: esig K}, env_t V -> forall k, V k -> env_t V;
-    create: forall {V: esig K}, forall (fn: forall k : K, V k), env_t V;
-    get_put_eq: forall {V: esig K} (ev: env_t V) k v, getenv (putenv ev k v) k = v;
-    get_put_neq: forall {V: esig K} (ev: env_t V) k k' v, k <> k' -> getenv (putenv ev k v) k' = getenv ev k';
-    fold_right: forall {V: esig K}, forall {T} (fn: forall k, V k -> T -> T) (ev: env_t V) (t0: T), T }.
+    create: forall {V: esig K} (fn: forall (k: K), V k), env_t V;
+    fold_right: forall {V: esig K} {T} (fn: forall k, V k -> T -> T) (ev: env_t V) (t0: T), T;
+    create_funext: forall {V: esig K} (fn1 fn2: forall k : K, V k),
+        (forall k, fn1 k = fn2 k) -> create fn1 = create fn2;
+    (* This axiom could be relaxed by proving that interp_rule is a
+       morphism wrt getenv-equivalence. *)
+    create_getenv_id: forall {V: esig K} (ev: env_t V),
+        create (getenv ev) = ev;
+    getenv_create: forall {V: esig K} (fn: forall k : K, V k) k,
+        getenv (create fn) k = fn k;
+    get_put_eq: forall {V: esig K} (ev: env_t V) k v,
+        getenv (putenv ev k v) k = v;
+    get_put_neq: forall {V: esig K} (ev: env_t V) k k' v,
+        k <> k' -> getenv (putenv ev k v) k' = getenv ev k' }.
 Arguments Env: clear implicits.
+
+Definition zip {K} {E: Env K} {V1 V2: esig K} (ev1: E.(env_t) V1) (ev2: E.(env_t) V2)
+  : E.(env_t) (fun k => V1 k * V2 k)%type :=
+  E.(create) (fun k => (E.(getenv) ev1 k, E.(getenv) ev2 k)).
+
+Definition map2 {K} (E: Env K) {V1 V2 V3: esig K} (fn: forall k, V1 k -> V2 k -> V3 k)
+           (ev1: E.(env_t) V1) (ev2: E.(env_t) V2)
+  : E.(env_t) V3 :=
+  E.(create) (fun k => fn k (E.(getenv) ev1 k) (E.(getenv) ev2 k)).
 
 Class FiniteType {T} :=
   { finite_elems: list T;
@@ -140,9 +189,12 @@ Definition ContextEnv {K} `{FiniteType K}: Env K.
   unshelve refine {| env_t V := context V finite_elems;
                      getenv {V} ctx k := cassoc (finite_index k) ctx;
                      putenv {V} ctx k v := creplace (finite_index k) v ctx;
-                     create {V} fn := ccreate finite_elems fn;
+                     create {V} fn := ccreate finite_elems (fun k _ => fn k);
                      fold_right {V T} (f: forall k: K, V k -> T -> T) ctx (t0: T) :=
                        List.fold_right (fun (k: K) (t: T) => f k (cassoc (finite_index k) ctx) t) t0 finite_elems |}.
+  - intros; apply ccreate_funext; eauto.
+  - 
+  - intros; apply cassoc_ccreate.
   - intros; apply cassoc_creplace_eq.
   - intros; apply cassoc_creplace_neq; eassumption.
 Defined.
@@ -168,193 +220,3 @@ Ltac FiniteType_t :=
   end.
 
 Hint Extern 2 (FiniteType _) => FiniteType_t : typeclass_instances.
-
-(* Create HintDb types discriminated. *)
-
-(* Hint Extern 1 => unfold not in *: types. *)
-
-(* Record fenv {Key Value: Type} := *)
-(*   { fn :> Key -> Value -> Prop; *)
-(*     uniq: forall k v v', fn k v -> fn k v' -> v = v' }. *)
-
-(* Arguments fenv: clear implicits. *)
-(* Hint Resolve @uniq : types. *)
-
-(* Definition fenv_nil {Key Value: Type} : fenv Key Value := *)
-(*   {| fn k v := False; *)
-(*      uniq := ltac:(cbv in *; tauto) |}. *)
-
-(* Definition fenv_add {Key Value: Type} (env: fenv Key Value) (k: Key) (v: Value) : fenv Key Value. *)
-(*   refine {| fn := (fun k' v' => (k = k' /\ v = v') \/ (k <> k' /\ env.(fn) k' v')) |}; *)
-(*     abstract (destruct env; intuition (subst; eauto with types)). *)
-(* Defined. *)
-
-(* Definition fenv_le {Key Value: Type} (cmp : Value -> Value -> Prop) (Gamma Gamma': fenv Key Value) := *)
-(*   forall k v, Gamma k v -> exists v', Gamma' k v' /\ cmp v v'. *)
-
-(* Class Env {K R: Type}: Type := *)
-(*   { env_t: Type; *)
-(*     env_nil: env_t; *)
-(*     getenv: env_t -> K -> option R; *)
-(*     putenv: env_t -> K -> R -> env_t; *)
-(*     getenv_nil: forall k, getenv env_nil k = None; *)
-(*     get_put_eq: forall ev k v, getenv (putenv ev k v) k = Some v; *)
-(*     get_put_neq: forall ev k k' v, k <> k' -> getenv (putenv ev k v) k' = getenv ev k'; *)
-(*     get_put_Some: forall ev k k' v v', *)
-(*         getenv (putenv ev k v) k' = Some v' <-> *)
-(*         k = k' /\ v = v' \/ k <> k' /\ getenv ev k' = Some v'; *)
-(*     get_put_None: forall ev k k' v, *)
-(*         getenv (putenv ev k v) k' = None <-> *)
-(*         k <> k' /\ getenv ev k' = None *)
-(*   }. *)
-(* Arguments Env : clear implicits. *)
-(* Arguments env_t {_ _}. *)
-
-(* Instance EqEnv {K R: Type} (eqdec: forall k k': K, {k = k'} + {k <> k'}) : Env K R. *)
-(* Proof. *)
-(*   refine ({| env_t := list (K * R); *)
-(*              env_nil := nil; *)
-(*              getenv e k := *)
-(*                match List.find (fun '(k', v) => if eqdec k k' then true else false) e with *)
-(*                | Some (_, v) => Some v *)
-(*                | None => None *)
-(*                end; *)
-(*              putenv e k v := cons (k, v) e |}); intros. *)
-(*   - abstract (reflexivity). *)
-(*   - abstract (cbn; destruct eqdec; congruence). *)
-(*   - abstract (cbn; destruct eqdec; congruence). *)
-(*   - abstract (cbn; destruct eqdec; subst; split; *)
-(*               intuition; repeat cleanup_step; eauto; congruence). *)
-(*   - abstract (cbn; destruct eqdec; subst; split; *)
-(*               intuition; repeat cleanup_step; eauto; congruence). *)
-(* Defined. *)
-
-(* Scheme Equality for string. *)
-(* Instance StringEnv (R: Type) : Env string R := EqEnv string_eq_dec. *)
-(* Instance NatEnv (R: Type) : Env nat R := EqEnv PeanoNat.Nat.eq_dec. *)
-
-(* Section EnvRel. *)
-(*   Context {K R R': Type} {Env: Env K R}. *)
-(*   Context (f: R -> R'). *)
-
-(*   Definition env_related (Gamma: fenv K R') (gamma: env_t Env) := *)
-(*     (forall var v, getenv gamma var = Some v -> Gamma var (f v)) /\ *)
-(*     (forall var, getenv gamma var = None -> forall tau, not (Gamma var tau)). *)
-
-(*   Lemma env_related_putenv: *)
-(*     forall (Gamma: fenv K R') (gamma: env_t _) *)
-(*       (k: K) (v': R') (v: R), *)
-(*       f v = v' -> *)
-(*       env_related Gamma gamma -> *)
-(*       env_related (fenv_add Gamma k v') (putenv gamma k v). *)
-(*   Proof. *)
-(*     unfold env_related; cbn. intros * ? (H & H') **. *)
-(*     split; intros; [ *)
-(*       pose proof (and_fst (get_put_Some _ _ _ _ _) ltac:(eassumption)) | *)
-(*       pose proof (and_fst (get_put_None _ _ _ _) ltac:(eassumption)) *)
-(*     ]; firstorder (subst; eauto). *)
-(*   Qed. *)
-
-(*   Lemma env_related_getenv_Some: *)
-(*     forall (Gamma: fenv K R') (k: K) (gamma: env_t _), *)
-(*       env_related Gamma gamma -> *)
-(*       forall v: R, *)
-(*         getenv gamma k = Some v -> *)
-(*         Gamma k (f v). *)
-(*   Proof. firstorder. Qed. *)
-
-(*   Lemma env_related_getenv_None: *)
-(*     forall (Gamma: fenv K R') (k: K) (gamma: env_t _), *)
-(*       env_related Gamma gamma -> *)
-(*       getenv gamma k = None -> *)
-(*       forall v', Gamma k v' -> False. *)
-(*   Proof. firstorder. Qed. *)
-
-(*   Definition tenv_of_env (ev: env_t Env): fenv K R'. *)
-(*     refine {| fn k v' := exists v, getenv ev k = Some v /\ v' = f v |}. *)
-(*     abstract (intros * (? & Heq & Hfeq) (? & Heq' & Hfeq'); subst; *)
-(*               rewrite Heq in Heq'; inversion Heq'; eauto). *)
-(*   Defined. *)
-
-(*   Lemma tenv_of_env_related : *)
-(*     forall (ev: env_t Env), *)
-(*       env_related (tenv_of_env ev) ev. *)
-(*   Proof. *)
-(*     intros; unfold env_related, tenv_of_env, not; cbn; split. *)
-(*     - firstorder. *)
-(*     - intros * Heq * Hex; rewrite Heq in Hex; *)
-(*         firstorder discriminate. *)
-(*   Qed. *)
-
-(*   Lemma tenv_of_env_nil : *)
-(*     env_related fenv_nil env_nil. *)
-(*     unfold env_related, fenv_nil; cbn; split; intros. *)
-(*     - rewrite getenv_nil in H; discriminate. *)
-(*     - tauto. *)
-(*   Qed. *)
-(* End EnvRel. *)
-
-(* Section FEnvRel. *)
-(*   Context {K R: Type} {Env: Env K R}. *)
-
-(*   Definition fenv_related (Gamma: fenv K R) (gamma: env_t Env) := *)
-(*     forall var v, Gamma var v <-> getenv gamma var = Some v. *)
-
-(*   Lemma fenv_related_putenv: *)
-(*     forall (Gamma: fenv K R) (gamma: env_t _) *)
-(*       (k: K) (v: R), *)
-(*       fenv_related Gamma gamma -> *)
-(*       fenv_related (fenv_add Gamma k v) (putenv gamma k v). *)
-(*   Proof. *)
-(*     unfold fenv_related; cbn; intros * H **. *)
-(*     rewrite get_put_Some, <- H. *)
-(*     reflexivity. *)
-(*   Qed. *)
-
-(*   Lemma fenv_related_getenv_Some: *)
-(*     forall (Gamma: fenv K R) (k: K) (gamma: env_t _), *)
-(*       fenv_related Gamma gamma -> *)
-(*       forall v: R, *)
-(*         Gamma k v -> getenv gamma k = Some v. *)
-(*   Proof. firstorder. Qed. *)
-
-(*   Lemma fenv_related_getenv_None: *)
-(*     forall (Gamma: fenv K R) (k: K) (gamma: env_t _), *)
-(*       fenv_related Gamma gamma -> *)
-(*       (forall v', Gamma k v' -> False) -> *)
-(*       getenv gamma k = None. *)
-(*   Proof. firstorder. *)
-(*      destruct getenv eqn:Heq. *)
-(*      - apply H in Heq; exfalso; eauto. *)
-(*      - reflexivity. *)
-(*   Qed. *)
-
-(*   Lemma tenv_of_env_frelated : *)
-(*     forall (ev: env_t Env), *)
-(*       fenv_related (tenv_of_env id ev) ev. *)
-(*   Proof. *)
-(*     intros; unfold fenv_related, tenv_of_env, id; cbn; firstorder (subst; eauto). *)
-(*   Qed. *)
-(* End FEnvRel. *)
-
-(* Lemma fenv_le_refl {Key Value: Type}: *)
-(*   forall (cmp: _ -> _ -> Prop) (Gamma : fenv Key Value), *)
-(*     (forall x, cmp x x) -> *)
-(*     fenv_le cmp Gamma Gamma. *)
-(* Proof. *)
-(*   firstorder. *)
-(* Qed. *)
-
-(* Hint Resolve fenv_le_refl : types. *)
-
-(* Lemma fenv_add_increasing {Key Value: Type}: *)
-(*   forall (cmp: _ -> _ -> Prop) (Gamma1 : fenv Key Value) (var : Key) (tau tau' : Value) (Gamma2 : fenv Key Value), *)
-(*     cmp tau tau' -> *)
-(*     fenv_le cmp Gamma1 Gamma2 -> *)
-(*     fenv_le cmp (fenv_add Gamma1 var tau) (fenv_add Gamma2 var tau'). *)
-(* Proof. *)
-(*   unfold fenv_le, fenv_add; simpl; firstorder (subst; eauto with types). *)
-(* Qed. *)
-
-(* Hint Resolve fenv_add_increasing : types. *)
-
